Update get_conv_case to directly use dvalue_byte serialization instead of going through uvalues.
- Separate dvalue_byte into its own module.

src/coq/Handlers/Concretization.v
@@ -68,6 +68,7 @@ Module Type ConcretizationBase (LP : LLVMParams) (MP : MemoryParams LP) (Byte : 
   Import GEP.
   Import SIZEOF.
   Import Events.
+  Import DVALUE_BYTES.
 
   Module MemHelpers := MemoryHelpers LP MP Byte.
   Import MemHelpers.
@@ -101,7 +102,6 @@ Module Type ConcretizationBase (LP : LLVMParams) (MP : MemoryParams LP) (Byte : 
         as would be natural, due to the [Int2Ptr] and [Ptr2Int] cases. At those types, the conversion
         needs to cast between integers and pointers, which depends on the memory model.
      *)
-
     Definition get_conv_case conv (t1:dtyp) (x:dvalue) (t2:dtyp) : conv_case :=
       match conv with
       | Trunc =>
@@ -110,19 +110,19 @@ Module Type ConcretizationBase (LP : LLVMParams) (MP : MemoryParams LP) (Byte : 
         | DTYPE_I 16, DVALUE_I16 i1, DTYPE_I 1
         | DTYPE_I 32, DVALUE_I32 i1, DTYPE_I 1
         | DTYPE_I 64, DVALUE_I64 i1, DTYPE_I 1 =>
-          Conv_Pure (UVALUE_I1 (repr (unsigned i1)))
+          Conv_Pure (DVALUE_I1 (repr (unsigned i1)))
 
         | DTYPE_I 16, DVALUE_I16 i1, DTYPE_I 8
         | DTYPE_I 32, DVALUE_I32 i1, DTYPE_I 8
         | DTYPE_I 64, DVALUE_I64 i1, DTYPE_I 8 =>
-          Conv_Pure (UVALUE_I8 (repr (unsigned i1)))
+          Conv_Pure (DVALUE_I8 (repr (unsigned i1)))
 
         | DTYPE_I 32, DVALUE_I32 i1, DTYPE_I 16
         | DTYPE_I 64, DVALUE_I64 i1, DTYPE_I 16 =>
-          Conv_Pure (UVALUE_I16 (repr (unsigned i1)))
+          Conv_Pure (DVALUE_I16 (repr (unsigned i1)))
 
         | DTYPE_I 64, DVALUE_I64 i1, DTYPE_I 32 =>
-          Conv_Pure (UVALUE_I32 (repr (unsigned i1)))
+          Conv_Pure (DVALUE_I32 (repr (unsigned i1)))
 
         | DTYPE_I 8, DVALUE_Poison t, DTYPE_I 1
         | DTYPE_I 16, DVALUE_Poison t, DTYPE_I 1
@@ -133,7 +133,7 @@ Module Type ConcretizationBase (LP : LLVMParams) (MP : MemoryParams LP) (Byte : 
         | DTYPE_I 64, DVALUE_Poison t, DTYPE_I 1
         | DTYPE_I 64, DVALUE_Poison t, DTYPE_I 8
         | DTYPE_I 64, DVALUE_Poison t, DTYPE_I 32 =>
-          Conv_Pure (UVALUE_Poison t)
+          Conv_Pure (DVALUE_Poison t)
 
         | _, _, _ => Conv_Illegal "ill-typed conv"
         end
@@ -141,22 +141,22 @@ Module Type ConcretizationBase (LP : LLVMParams) (MP : MemoryParams LP) (Byte : 
       | Zext =>
         match t1, x, t2 with
         | DTYPE_I 1, DVALUE_I1 i1, DTYPE_I 8 =>
-          Conv_Pure (UVALUE_I8 (repr (unsigned i1)))
+          Conv_Pure (DVALUE_I8 (repr (unsigned i1)))
 
         | DTYPE_I 1, DVALUE_I1 i1, DTYPE_I 16
         | DTYPE_I 8, DVALUE_I8 i1, DTYPE_I 16 =>
-          Conv_Pure (UVALUE_I16 (repr (unsigned i1)))
+          Conv_Pure (DVALUE_I16 (repr (unsigned i1)))
 
         | DTYPE_I 1, DVALUE_I1 i1, DTYPE_I 32
         | DTYPE_I 8, DVALUE_I8 i1, DTYPE_I 32
         | DTYPE_I 16, DVALUE_I16 i1, DTYPE_I 32 =>
-          Conv_Pure (UVALUE_I32 (repr (unsigned i1)))
+          Conv_Pure (DVALUE_I32 (repr (unsigned i1)))
 
         | DTYPE_I 1, DVALUE_I1 i1, DTYPE_I 64
         | DTYPE_I 8, DVALUE_I8 i1, DTYPE_I 64
         | DTYPE_I 16, DVALUE_I16 i1, DTYPE_I 64
         | DTYPE_I 32, DVALUE_I32 i1, DTYPE_I 64 =>
-          Conv_Pure (UVALUE_I64 (repr (unsigned i1)))
+          Conv_Pure (DVALUE_I64 (repr (unsigned i1)))
 
         | DTYPE_I 1, DVALUE_Poison t, DTYPE_I 8
         | DTYPE_I 1, DVALUE_Poison t, DTYPE_I 16
@@ -168,7 +168,7 @@ Module Type ConcretizationBase (LP : LLVMParams) (MP : MemoryParams LP) (Byte : 
         | DTYPE_I 16, DVALUE_Poison t, DTYPE_I 32
         | DTYPE_I 16, DVALUE_Poison t, DTYPE_I 64
         | DTYPE_I 32, DVALUE_Poison t, DTYPE_I 64 =>
-          Conv_Pure (UVALUE_Poison t)
+          Conv_Pure (DVALUE_Poison t)
 
         | _, _, _ => Conv_Illegal "ill-typed conv"
         end
@@ -176,22 +176,22 @@ Module Type ConcretizationBase (LP : LLVMParams) (MP : MemoryParams LP) (Byte : 
       | Sext =>
         match t1, x, t2 with
         | DTYPE_I 1, DVALUE_I1 i1, DTYPE_I 8 =>
-          Conv_Pure (UVALUE_I8 (repr (signed i1)))
+          Conv_Pure (DVALUE_I8 (repr (signed i1)))
 
         | DTYPE_I 1, DVALUE_I1 i1, DTYPE_I 16
         | DTYPE_I 8, DVALUE_I8 i1, DTYPE_I 16 =>
-          Conv_Pure (UVALUE_I16 (repr (signed i1)))
+          Conv_Pure (DVALUE_I16 (repr (signed i1)))
 
         | DTYPE_I 1, DVALUE_I1 i1, DTYPE_I 32
         | DTYPE_I 8, DVALUE_I8 i1, DTYPE_I 32
         | DTYPE_I 16, DVALUE_I16 i1, DTYPE_I 32 =>
-          Conv_Pure (UVALUE_I32 (repr (signed i1)))
+          Conv_Pure (DVALUE_I32 (repr (signed i1)))
 
         | DTYPE_I 1, DVALUE_I1 i1, DTYPE_I 64
         | DTYPE_I 8, DVALUE_I8 i1, DTYPE_I 64
         | DTYPE_I 16, DVALUE_I16 i1, DTYPE_I 64
         | DTYPE_I 32, DVALUE_I32 i1, DTYPE_I 64 =>
-          Conv_Pure (UVALUE_I64 (repr (signed i1)))
+          Conv_Pure (DVALUE_I64 (repr (signed i1)))
 
         | DTYPE_I 1, DVALUE_Poison t, DTYPE_I 8
         | DTYPE_I 1, DVALUE_Poison t, DTYPE_I 16
@@ -203,29 +203,27 @@ Module Type ConcretizationBase (LP : LLVMParams) (MP : MemoryParams LP) (Byte : 
         | DTYPE_I 16, DVALUE_Poison t, DTYPE_I 32
         | DTYPE_I 16, DVALUE_Poison t, DTYPE_I 64
         | DTYPE_I 32, DVALUE_Poison t, DTYPE_I 64 =>
-          Conv_Pure (UVALUE_Poison t)
+          Conv_Pure (DVALUE_Poison t)
 
         | _, _, _ => Conv_Illegal "ill-typed conv"
         end
 
       | Bitcast =>
           if dtyp_eqb t1 t2
-          then Conv_Pure (dvalue_to_uvalue x)
+          then Conv_Pure x
           else if bit_sizeof_dtyp t1 =? bit_sizeof_dtyp t2
                then
-                 let bytes := evalStateT (serialize_sbytes (dvalue_to_uvalue x) t1) 0%N in
-                 match unIdent (unEitherT (unEitherT (unEitherT (unERR_UB_OOM bytes)))) with
+                 let bytes := dvalue_to_dvalue_bytes x t1 in
+                 let dv_conv := ErrOOMPoison_handle_poison_and_oom DVALUE_Poison (@dvalue_bytes_to_dvalue ErrOOMPoison _ _ _ _ bytes t2) in
+                 match unIdent (unEitherT (unEitherT (unEitherT (unERR_UB_OOM dv_conv)))) with
                  | inl (OOM_message oom) =>
                      Conv_Illegal ("Bitcast OOM: " ++ oom)
                  | inr (inl (UB_message ub)) =>
                      Conv_Illegal ("Bitcast UB: " ++ ub)
                  | inr (inr (inl (ERR_message err))) =>
                      Conv_Illegal ("Bitcast Error: " ++ err)
-                 | inr (inr (inr bytes)) =>
-                     match deserialize_sbytes bytes t2 with
-                     | inl msg => Conv_Illegal ("Bitcast failed: " ++ msg)
-                     | inr uv => Conv_Pure uv
-                     end
+                 | inr (inr (inr dv)) =>
+                     Conv_Pure dv
                  end
                else Conv_Illegal "unequal bitsize in cast"
 
@@ -236,14 +234,14 @@ Module Type ConcretizationBase (LP : LLVMParams) (MP : MemoryParams LP) (Byte : 
         | DTYPE_I 16, DVALUE_I16 i1, DTYPE_Float
         | DTYPE_I 32, DVALUE_I32 i1, DTYPE_Float
         | DTYPE_I 64, DVALUE_I64 i1, DTYPE_Float =>
-          Conv_Pure (UVALUE_Float (Float32.of_intu (repr (unsigned i1))))
+          Conv_Pure (DVALUE_Float (Float32.of_intu (repr (unsigned i1))))
 
         | DTYPE_I 1, DVALUE_I1 i1, DTYPE_Double
         | DTYPE_I 8, DVALUE_I8 i1, DTYPE_Double
         | DTYPE_I 16, DVALUE_I16 i1, DTYPE_Double
         | DTYPE_I 32, DVALUE_I32 i1, DTYPE_Double
         | DTYPE_I 64, DVALUE_I64 i1, DTYPE_Double =>
-          Conv_Pure (UVALUE_Double (Float.of_longu (repr (unsigned i1))))
+          Conv_Pure (DVALUE_Double (Float.of_longu (repr (unsigned i1))))
 
         | DTYPE_I 1, DVALUE_Poison t, DTYPE_Float
         | DTYPE_I 8, DVALUE_Poison t, DTYPE_Float
@@ -255,7 +253,7 @@ Module Type ConcretizationBase (LP : LLVMParams) (MP : MemoryParams LP) (Byte : 
         | DTYPE_I 16, DVALUE_Poison t, DTYPE_Double
         | DTYPE_I 32, DVALUE_Poison t, DTYPE_Double
         | DTYPE_I 64, DVALUE_Poison t, DTYPE_Double =>
-          Conv_Pure (UVALUE_Poison t)
+          Conv_Pure (DVALUE_Poison t)
 
         | _, _, _ => Conv_Illegal "ill-typed Uitofp"
         end
@@ -267,14 +265,14 @@ Module Type ConcretizationBase (LP : LLVMParams) (MP : MemoryParams LP) (Byte : 
         | DTYPE_I 16, DVALUE_I16 i1, DTYPE_Float
         | DTYPE_I 32, DVALUE_I32 i1, DTYPE_Float
         | DTYPE_I 64, DVALUE_I64 i1, DTYPE_Float =>
-          Conv_Pure (UVALUE_Float (Float32.of_intu (repr (signed i1))))
+          Conv_Pure (DVALUE_Float (Float32.of_intu (repr (signed i1))))
 
         | DTYPE_I 1, DVALUE_I1 i1, DTYPE_Double
         | DTYPE_I 8, DVALUE_I8 i1, DTYPE_Double
         | DTYPE_I 16, DVALUE_I16 i1, DTYPE_Double
         | DTYPE_I 32, DVALUE_I32 i1, DTYPE_Double
         | DTYPE_I 64, DVALUE_I64 i1, DTYPE_Double =>
-          Conv_Pure (UVALUE_Double (Float.of_longu (repr (signed i1))))
+          Conv_Pure (DVALUE_Double (Float.of_longu (repr (signed i1))))
 
         | DTYPE_I 1, DVALUE_Poison t, DTYPE_Float
         | DTYPE_I 8, DVALUE_Poison t, DTYPE_Float
@@ -286,7 +284,7 @@ Module Type ConcretizationBase (LP : LLVMParams) (MP : MemoryParams LP) (Byte : 
         | DTYPE_I 16, DVALUE_Poison t, DTYPE_Double
         | DTYPE_I 32, DVALUE_Poison t, DTYPE_Double
         | DTYPE_I 64, DVALUE_Poison t, DTYPE_Double =>
-          Conv_Pure (UVALUE_Poison t)
+          Conv_Pure (DVALUE_Poison t)
 
         | _, _, _ => Conv_Illegal "ill-typed Sitofp"
         end
@@ -375,7 +373,7 @@ Module Type ConcretizationBase (LP : LLVMParams) (MP : MemoryParams LP) (Byte : 
         | UVALUE_Conversion conv t_from v t_to =>
             dv <- concretize_uvalueM M undef_handler ERR_M lift_ue v;;
             match get_conv_case conv t_from dv t_to with
-            | Conv_Pure x => concretize_uvalueM M undef_handler ERR_M lift_ue x
+            | Conv_Pure x => ret x
             | Conv_ItoP x =>
                 match int_to_ptr (dvalue_int_unsigned x) wildcard_prov with
                 | NoOom a =>
@@ -676,6 +674,7 @@ Module MakeBase (LP : LLVMParams) (MP : MemoryParams LP) (Byte : ByteModule LP.A
   Import ITOP.
   Import DV.
   Import GEP.
+  Import DVALUE_BYTES.
   Open Scope list.
 
   Export Byte.
@@ -731,19 +730,19 @@ Module MakeBase (LP : LLVMParams) (MP : MemoryParams LP) (Byte : ByteModule LP.A
         | DTYPE_I 16, DVALUE_I16 i1, DTYPE_I 1
         | DTYPE_I 32, DVALUE_I32 i1, DTYPE_I 1
         | DTYPE_I 64, DVALUE_I64 i1, DTYPE_I 1 =>
-          Conv_Pure (UVALUE_I1 (repr (unsigned i1)))
+          Conv_Pure (DVALUE_I1 (repr (unsigned i1)))
 
         | DTYPE_I 16, DVALUE_I16 i1, DTYPE_I 8
         | DTYPE_I 32, DVALUE_I32 i1, DTYPE_I 8
         | DTYPE_I 64, DVALUE_I64 i1, DTYPE_I 8 =>
-          Conv_Pure (UVALUE_I8 (repr (unsigned i1)))
+          Conv_Pure (DVALUE_I8 (repr (unsigned i1)))
 
         | DTYPE_I 32, DVALUE_I32 i1, DTYPE_I 16
         | DTYPE_I 64, DVALUE_I64 i1, DTYPE_I 16 =>
-          Conv_Pure (UVALUE_I16 (repr (unsigned i1)))
+          Conv_Pure (DVALUE_I16 (repr (unsigned i1)))
 
         | DTYPE_I 64, DVALUE_I64 i1, DTYPE_I 32 =>
-          Conv_Pure (UVALUE_I32 (repr (unsigned i1)))
+          Conv_Pure (DVALUE_I32 (repr (unsigned i1)))
 
         | DTYPE_I 8, DVALUE_Poison t, DTYPE_I 1
         | DTYPE_I 16, DVALUE_Poison t, DTYPE_I 1
@@ -754,7 +753,7 @@ Module MakeBase (LP : LLVMParams) (MP : MemoryParams LP) (Byte : ByteModule LP.A
         | DTYPE_I 64, DVALUE_Poison t, DTYPE_I 1
         | DTYPE_I 64, DVALUE_Poison t, DTYPE_I 8
         | DTYPE_I 64, DVALUE_Poison t, DTYPE_I 32 =>
-          Conv_Pure (UVALUE_Poison t)
+          Conv_Pure (DVALUE_Poison t)
 
         | _, _, _ => Conv_Illegal "ill-typed conv"
         end
@@ -762,22 +761,22 @@ Module MakeBase (LP : LLVMParams) (MP : MemoryParams LP) (Byte : ByteModule LP.A
       | Zext =>
         match t1, x, t2 with
         | DTYPE_I 1, DVALUE_I1 i1, DTYPE_I 8 =>
-          Conv_Pure (UVALUE_I8 (repr (unsigned i1)))
+          Conv_Pure (DVALUE_I8 (repr (unsigned i1)))
 
         | DTYPE_I 1, DVALUE_I1 i1, DTYPE_I 16
         | DTYPE_I 8, DVALUE_I8 i1, DTYPE_I 16 =>
-          Conv_Pure (UVALUE_I16 (repr (unsigned i1)))
+          Conv_Pure (DVALUE_I16 (repr (unsigned i1)))
 
         | DTYPE_I 1, DVALUE_I1 i1, DTYPE_I 32
         | DTYPE_I 8, DVALUE_I8 i1, DTYPE_I 32
         | DTYPE_I 16, DVALUE_I16 i1, DTYPE_I 32 =>
-          Conv_Pure (UVALUE_I32 (repr (unsigned i1)))
+          Conv_Pure (DVALUE_I32 (repr (unsigned i1)))
 
         | DTYPE_I 1, DVALUE_I1 i1, DTYPE_I 64
         | DTYPE_I 8, DVALUE_I8 i1, DTYPE_I 64
         | DTYPE_I 16, DVALUE_I16 i1, DTYPE_I 64
         | DTYPE_I 32, DVALUE_I32 i1, DTYPE_I 64 =>
-          Conv_Pure (UVALUE_I64 (repr (unsigned i1)))
+          Conv_Pure (DVALUE_I64 (repr (unsigned i1)))
 
         | DTYPE_I 1, DVALUE_Poison t, DTYPE_I 8
         | DTYPE_I 1, DVALUE_Poison t, DTYPE_I 16
@@ -789,7 +788,7 @@ Module MakeBase (LP : LLVMParams) (MP : MemoryParams LP) (Byte : ByteModule LP.A
         | DTYPE_I 16, DVALUE_Poison t, DTYPE_I 32
         | DTYPE_I 16, DVALUE_Poison t, DTYPE_I 64
         | DTYPE_I 32, DVALUE_Poison t, DTYPE_I 64 =>
-          Conv_Pure (UVALUE_Poison t)
+          Conv_Pure (DVALUE_Poison t)
 
         | _, _, _ => Conv_Illegal "ill-typed conv"
         end
@@ -797,22 +796,22 @@ Module MakeBase (LP : LLVMParams) (MP : MemoryParams LP) (Byte : ByteModule LP.A
       | Sext =>
         match t1, x, t2 with
         | DTYPE_I 1, DVALUE_I1 i1, DTYPE_I 8 =>
-          Conv_Pure (UVALUE_I8 (repr (signed i1)))
+          Conv_Pure (DVALUE_I8 (repr (signed i1)))
 
         | DTYPE_I 1, DVALUE_I1 i1, DTYPE_I 16
         | DTYPE_I 8, DVALUE_I8 i1, DTYPE_I 16 =>
-          Conv_Pure (UVALUE_I16 (repr (signed i1)))
+          Conv_Pure (DVALUE_I16 (repr (signed i1)))
 
         | DTYPE_I 1, DVALUE_I1 i1, DTYPE_I 32
         | DTYPE_I 8, DVALUE_I8 i1, DTYPE_I 32
         | DTYPE_I 16, DVALUE_I16 i1, DTYPE_I 32 =>
-          Conv_Pure (UVALUE_I32 (repr (signed i1)))
+          Conv_Pure (DVALUE_I32 (repr (signed i1)))
 
         | DTYPE_I 1, DVALUE_I1 i1, DTYPE_I 64
         | DTYPE_I 8, DVALUE_I8 i1, DTYPE_I 64
         | DTYPE_I 16, DVALUE_I16 i1, DTYPE_I 64
         | DTYPE_I 32, DVALUE_I32 i1, DTYPE_I 64 =>
-          Conv_Pure (UVALUE_I64 (repr (signed i1)))
+          Conv_Pure (DVALUE_I64 (repr (signed i1)))
 
         | DTYPE_I 1, DVALUE_Poison t, DTYPE_I 8
         | DTYPE_I 1, DVALUE_Poison t, DTYPE_I 16
@@ -824,29 +823,27 @@ Module MakeBase (LP : LLVMParams) (MP : MemoryParams LP) (Byte : ByteModule LP.A
         | DTYPE_I 16, DVALUE_Poison t, DTYPE_I 32
         | DTYPE_I 16, DVALUE_Poison t, DTYPE_I 64
         | DTYPE_I 32, DVALUE_Poison t, DTYPE_I 64 =>
-          Conv_Pure (UVALUE_Poison t)
+          Conv_Pure (DVALUE_Poison t)
 
         | _, _, _ => Conv_Illegal "ill-typed conv"
         end
 
       | Bitcast =>
           if dtyp_eqb t1 t2
-          then Conv_Pure (dvalue_to_uvalue x)
+          then Conv_Pure x
           else if bit_sizeof_dtyp t1 =? bit_sizeof_dtyp t2
                then
-                 let bytes := evalStateT (serialize_sbytes (dvalue_to_uvalue x) t1) 0%N in
-                 match unIdent (unEitherT (unEitherT (unEitherT (unERR_UB_OOM bytes)))) with
+                 let bytes := dvalue_to_dvalue_bytes x t1 in
+                 let dv_conv := ErrOOMPoison_handle_poison_and_oom DVALUE_Poison (@dvalue_bytes_to_dvalue ErrOOMPoison _ _ _ _ bytes t2) in
+                 match unIdent (unEitherT (unEitherT (unEitherT (unERR_UB_OOM dv_conv)))) with
                  | inl (OOM_message oom) =>
                      Conv_Illegal ("Bitcast OOM: " ++ oom)
                  | inr (inl (UB_message ub)) =>
                      Conv_Illegal ("Bitcast UB: " ++ ub)
                  | inr (inr (inl (ERR_message err))) =>
                      Conv_Illegal ("Bitcast Error: " ++ err)
-                 | inr (inr (inr bytes)) =>
-                     match deserialize_sbytes bytes t2 with
-                     | inl msg => Conv_Illegal ("Bitcast failed: " ++ msg)
-                     | inr uv => Conv_Pure uv
-                     end
+                 | inr (inr (inr dv)) =>
+                     Conv_Pure dv
                  end
                else Conv_Illegal "unequal bitsize in cast"
 
@@ -857,14 +854,14 @@ Module MakeBase (LP : LLVMParams) (MP : MemoryParams LP) (Byte : ByteModule LP.A
         | DTYPE_I 16, DVALUE_I16 i1, DTYPE_Float
         | DTYPE_I 32, DVALUE_I32 i1, DTYPE_Float
         | DTYPE_I 64, DVALUE_I64 i1, DTYPE_Float =>
-          Conv_Pure (UVALUE_Float (Float32.of_intu (repr (unsigned i1))))
+          Conv_Pure (DVALUE_Float (Float32.of_intu (repr (unsigned i1))))
 
         | DTYPE_I 1, DVALUE_I1 i1, DTYPE_Double
         | DTYPE_I 8, DVALUE_I8 i1, DTYPE_Double
         | DTYPE_I 16, DVALUE_I16 i1, DTYPE_Double
         | DTYPE_I 32, DVALUE_I32 i1, DTYPE_Double
         | DTYPE_I 64, DVALUE_I64 i1, DTYPE_Double =>
-          Conv_Pure (UVALUE_Double (Float.of_longu (repr (unsigned i1))))
+          Conv_Pure (DVALUE_Double (Float.of_longu (repr (unsigned i1))))
 
         | DTYPE_I 1, DVALUE_Poison t, DTYPE_Float
         | DTYPE_I 8, DVALUE_Poison t, DTYPE_Float
@@ -876,7 +873,7 @@ Module MakeBase (LP : LLVMParams) (MP : MemoryParams LP) (Byte : ByteModule LP.A
         | DTYPE_I 16, DVALUE_Poison t, DTYPE_Double
         | DTYPE_I 32, DVALUE_Poison t, DTYPE_Double
         | DTYPE_I 64, DVALUE_Poison t, DTYPE_Double =>
-          Conv_Pure (UVALUE_Poison t)
+          Conv_Pure (DVALUE_Poison t)
 
         | _, _, _ => Conv_Illegal "ill-typed Uitofp"
         end
@@ -888,14 +885,14 @@ Module MakeBase (LP : LLVMParams) (MP : MemoryParams LP) (Byte : ByteModule LP.A
         | DTYPE_I 16, DVALUE_I16 i1, DTYPE_Float
         | DTYPE_I 32, DVALUE_I32 i1, DTYPE_Float
         | DTYPE_I 64, DVALUE_I64 i1, DTYPE_Float =>
-          Conv_Pure (UVALUE_Float (Float32.of_intu (repr (signed i1))))
+          Conv_Pure (DVALUE_Float (Float32.of_intu (repr (signed i1))))
 
         | DTYPE_I 1, DVALUE_I1 i1, DTYPE_Double
         | DTYPE_I 8, DVALUE_I8 i1, DTYPE_Double
         | DTYPE_I 16, DVALUE_I16 i1, DTYPE_Double
         | DTYPE_I 32, DVALUE_I32 i1, DTYPE_Double
         | DTYPE_I 64, DVALUE_I64 i1, DTYPE_Double =>
-          Conv_Pure (UVALUE_Double (Float.of_longu (repr (signed i1))))
+          Conv_Pure (DVALUE_Double (Float.of_longu (repr (signed i1))))
 
         | DTYPE_I 1, DVALUE_Poison t, DTYPE_Float
         | DTYPE_I 8, DVALUE_Poison t, DTYPE_Float
@@ -907,7 +904,7 @@ Module MakeBase (LP : LLVMParams) (MP : MemoryParams LP) (Byte : ByteModule LP.A
         | DTYPE_I 16, DVALUE_Poison t, DTYPE_Double
         | DTYPE_I 32, DVALUE_Poison t, DTYPE_Double
         | DTYPE_I 64, DVALUE_Poison t, DTYPE_Double =>
-          Conv_Pure (UVALUE_Poison t)
+          Conv_Pure (DVALUE_Poison t)
 
         | _, _, _ => Conv_Illegal "ill-typed Sitofp"
         end
@@ -1003,504 +1000,6 @@ Module MakeBase (LP : LLVMParams) (MP : MemoryParams LP) (Byte : ByteModule LP.A
   (* TODO: address termination checker here *)
   Unset Guard Checking.
   Section Concretize.
-
-
-    (* Convert a list of UVALUE_ExtractByte values into a dvalue of
-         a given type.
-
-         Assumes bytes are in little endian form...
-
-         Note: I believe this function has to be endianess aware.
-
-         This probably also needs to be mutually recursive with
-         concretize_uvalue...
-
-         Idea:
-
-         For each byte in the list, find uvalues that are from the
-         same store.
-
-         - Can I have bytes that are from the same store, but
-           different uvalues?  + Might not be possible, actually,
-           because if I store a concatbytes I get the old sids...  +
-           TODO: Getting the old sids might be a problem,
-           though. Should be new, but entangled wherever they were
-           entangled before. This needs to be changed in serialize...
-           * I.e., If I load bytes from one store, and then store them
-           beside them... It should have a different sid, allowing the
-           bytes from that store to vary independently.  * ALSO bytes
-           that are entangled should *stay* entangled.
-
-         The above is largely an issue with serialize_sbytes...
-
-         The idea here should be to take equal uvalues in our byte
-         list with the same sid and concretize the uvalue exactly
-         once.
-
-         After all uvalues in our list are concretized we then need to
-         convert the corresponding byte extractions into a single
-         dvalue.
-
-     *)
-
-    (* TODO: probably move this *)
-    (* TODO: Make these take endianess into account.
-
-         Can probably use bitwidth from VInt to do big-endian...
-     *)
-    Definition extract_byte_vint {I} `{VInt I} (i : I) (idx : Z) : Z
-      := unsigned (modu (shru i (repr (idx * 8))) (repr 256)).
-
-    Fixpoint concat_bytes_vint {I} `{VInt I} (bytes : list I) : I
-      := match bytes with
-         | [] => repr 0
-         | (byte::bytes) =>
-             add byte (shl (concat_bytes_vint bytes) (repr 8))
-         end.
-
-    (* TODO: Endianess *)
-    (* TODO: does this work correctly with negative x? *)
-    Definition extract_byte_Z (x : Z) (idx : Z) : Z
-      := (Z.shiftr x (idx * 8)) mod 256.
-
-    (* TODO: Endianess *)
-    Definition concat_bytes_Z_vint {I} `{VInt I} (bytes : list Z) : I
-      := concat_bytes_vint (map repr bytes).
-
-    (* TODO: Endianess *)
-    Fixpoint concat_bytes_Z (bytes : list Z) : Z
-      := match bytes with
-         | [] => 0
-         | (byte::bytes) =>
-             byte + (Z.shiftl (concat_bytes_Z bytes) 8)
-         end.
-
-    (* Walk through a list *)
-    (* Returns field index + number of bytes remaining *)
-    Fixpoint extract_field_byte_helper {M} `{Monad M} `{RAISE_ERROR M} (fields : list dtyp) (field_idx : N) (byte_idx : N) : M (dtyp * (N * N))%type
-      := match fields with
-         | [] =>
-             raise_error "No fields left for byte-indexing..."
-         | (x::xs) =>
-             let sz := sizeof_dtyp x
-             in if N.ltb byte_idx sz
-                then ret (x, (field_idx, byte_idx))
-                else extract_field_byte_helper xs (N.succ field_idx) (byte_idx - sz)
-         end.
-
-    Definition extract_field_byte {M} `{Monad M} `{RAISE_ERROR M} (fields : list dtyp) (byte_idx : N) : M (dtyp * (N * N))%type
-      := extract_field_byte_helper fields 0 byte_idx.
-
-    (* Need the type of the dvalue in order to know how big fields and array elements are.
-
-         It's not possible to use the dvalue alone, as DVALUE_Poison's
-         size depends on the type.
-     *)
-    Obligation Tactic := try Tactics.program_simpl; try solve [cbn; try lia | solve_dvalue_measure].
-    Program Fixpoint dvalue_extract_byte {M} `{Monad M} `{RAISE_ERROR M} `{RAISE_POISON M} `{RAISE_OOMABLE M} (dv : dvalue) (dt : dtyp) (idx : Z) {measure (dvalue_measure dv)} : M Z
-      := match dv with
-         | DVALUE_I1 x
-         | DVALUE_I8 x
-         | DVALUE_I16 x
-         | DVALUE_I32 x
-         | DVALUE_I64 x =>
-             ret (extract_byte_vint x idx)
-         | DVALUE_IPTR x =>
-             ret (extract_byte_Z (IP.to_Z x) idx)
-         | DVALUE_Addr addr =>
-             (* Note: this throws away provenance *)
-             ret (extract_byte_Z (ptr_to_int addr) idx)
-         | DVALUE_Float f =>
-             ret (extract_byte_Z (unsigned (Float32.to_bits f)) idx)
-         | DVALUE_Double d =>
-             ret (extract_byte_Z (unsigned (Float.to_bits d)) idx)
-         | DVALUE_Poison dt => raise_poison dt
-         | DVALUE_Oom dt => raise_oomable dt
-         | DVALUE_None =>
-             (* TODO: Not sure if this should be an error, poison, or what. *)
-             raise_error "dvalue_extract_byte on DVALUE_None"
-
-         (* TODO: Take padding into account. *)
-         | DVALUE_Struct fields =>
-             match dt with
-             | DTYPE_Struct dts =>
-                 (* Step to field which contains the byte we want *)
-                 '(fdt, (field_idx, byte_idx)) <- extract_field_byte dts (Z.to_N idx);;
-                 match List.nth_error fields (N.to_nat field_idx) with
-                 | Some f =>
-                     (* call dvalue_extract_byte recursively on the field *)
-                     dvalue_extract_byte f fdt (Z.of_N byte_idx )
-                 | None =>
-                     raise_error "dvalue_extract_byte: more fields in DVALUE_Struct than in dtyp."
-                 end
-             | _ => raise_error "dvalue_extract_byte: type mismatch on DVALUE_Struct."
-             end
-
-         | DVALUE_Packed_struct fields =>
-             match dt with
-             | DTYPE_Packed_struct dts =>
-                 (* Step to field which contains the byte we want *)
-                 '(fdt, (field_idx, byte_idx)) <- extract_field_byte dts (Z.to_N idx);;
-                 match List.nth_error fields (N.to_nat field_idx) with
-                 | Some f =>
-                     (* call dvalue_extract_byte recursively on the field *)
-                     dvalue_extract_byte f fdt (Z.of_N byte_idx )
-                 | None =>
-                     raise_error "dvalue_extract_byte: more fields in DVALUE_Packed_struct than in dtyp."
-                 end
-             | _ => raise_error "dvalue_extract_byte: type mismatch on DVALUE_Packed_struct."
-             end
-
-         | DVALUE_Array elts =>
-             match dt with
-             | DTYPE_Array sz dt =>
-                 let elmt_sz  := sizeof_dtyp dt in
-                 let elmt_idx := N.div (Z.to_N idx) elmt_sz in
-                 let byte_idx := (Z.to_N idx) mod elmt_sz in
-                 match List.nth_error elts (N.to_nat elmt_idx) with
-                 | Some elmt =>
-                     (* call dvalue_extract_byte recursively on the field *)
-                     dvalue_extract_byte elmt dt (Z.of_N byte_idx)
-                 | None =>
-                     raise_error "dvalue_extract_byte: more fields in dvalue than in dtyp."
-                 end
-             | _ =>
-                 raise_error "dvalue_extract_byte: type mismatch on DVALUE_Array."
-             end
-
-         | DVALUE_Vector elts =>
-             match dt with
-             | DTYPE_Vector sz dt =>
-                 let elmt_sz  := sizeof_dtyp dt in
-                 let elmt_idx := N.div (Z.to_N idx) elmt_sz in
-                 let byte_idx := (Z.to_N idx) mod elmt_sz in
-                 match List.nth_error elts (N.to_nat elmt_idx) with
-                 | Some elmt =>
-                     (* call dvalue_extract_byte recursively on the field *)
-                     dvalue_extract_byte elmt dt (Z.of_N byte_idx)
-                 | None =>
-                     raise_error "dvalue_extract_byte: more fields in dvalue than in dtyp."
-                 end
-             | _ =>
-                 raise_error "dvalue_extract_byte: type mismatch on DVALUE_Vector."
-             end
-         end.
-
-    Lemma dvalue_extract_byte_equation {M} `{HM: Monad M} `{RE: RAISE_ERROR M} `{RP: RAISE_POISON M} `{RO: RAISE_OOMABLE M} (dv : dvalue) (dt : dtyp) (idx : Z) :
-      @dvalue_extract_byte M HM RE RP RO dv dt idx =
-        match dv with
-        | DVALUE_I1 x
-        | DVALUE_I8 x
-        | DVALUE_I16 x
-        | DVALUE_I32 x
-        | DVALUE_I64 x =>
-            ret (extract_byte_vint x idx)
-        | DVALUE_IPTR x =>
-            ret (extract_byte_Z (IP.to_Z x) idx)
-        | DVALUE_Addr addr =>
-            (* Note: this throws away provenance *)
-            ret (extract_byte_Z (ptr_to_int addr) idx)
-        | DVALUE_Float f =>
-            ret (extract_byte_Z (unsigned (Float32.to_bits f)) idx)
-        | DVALUE_Double d =>
-            ret (extract_byte_Z (unsigned (Float.to_bits d)) idx)
-        | DVALUE_Poison dt => raise_poison dt
-        | DVALUE_Oom dt => raise_oomable dt
-        | DVALUE_None =>
-            (* TODO: Not sure if this should be an error, poison, or what. *)
-            raise_error "dvalue_extract_byte on DVALUE_None"
-
-        (* TODO: Take padding into account. *)
-        | DVALUE_Struct fields =>
-            match dt with
-            | DTYPE_Struct dts =>
-                (* Step to field which contains the byte we want *)
-                '(fdt, (field_idx, byte_idx)) <- extract_field_byte dts (Z.to_N idx);;
-                match List.nth_error fields (N.to_nat field_idx) with
-                | Some f =>
-                    (* call dvalue_extract_byte recursively on the field *)
-                    dvalue_extract_byte f fdt (Z.of_N byte_idx )
-                | None =>
-                    raise_error "dvalue_extract_byte: more fields in DVALUE_Struct than in dtyp."
-                end
-            | _ => raise_error "dvalue_extract_byte: type mismatch on DVALUE_Struct."
-            end
-
-        | DVALUE_Packed_struct fields =>
-            match dt with
-            | DTYPE_Packed_struct dts =>
-                (* Step to field which contains the byte we want *)
-                '(fdt, (field_idx, byte_idx)) <- extract_field_byte dts (Z.to_N idx);;
-                match List.nth_error fields (N.to_nat field_idx) with
-                | Some f =>
-                    (* call dvalue_extract_byte recursively on the field *)
-                    dvalue_extract_byte f fdt (Z.of_N byte_idx )
-                | None =>
-                    raise_error "dvalue_extract_byte: more fields in DVALUE_Packed_struct than in dtyp."
-                end
-            | _ => raise_error "dvalue_extract_byte: type mismatch on DVALUE_Packed_struct."
-            end
-
-        | DVALUE_Array elts =>
-            match dt with
-            | DTYPE_Array sz dt =>
-                let elmt_sz  := sizeof_dtyp dt in
-                let elmt_idx := N.div (Z.to_N idx) elmt_sz in
-                let byte_idx := (Z.to_N idx) mod elmt_sz in
-                match List.nth_error elts (N.to_nat elmt_idx) with
-                | Some elmt =>
-                    (* call dvalue_extract_byte recursively on the field *)
-                    dvalue_extract_byte elmt dt (Z.of_N byte_idx)
-                | None =>
-                    raise_error "dvalue_extract_byte: more fields in dvalue than in dtyp."
-                end
-            | _ =>
-                raise_error "dvalue_extract_byte: type mismatch on DVALUE_Array."
-            end
-
-        | DVALUE_Vector elts =>
-            match dt with
-            | DTYPE_Vector sz dt =>
-                let elmt_sz  := sizeof_dtyp dt in
-                let elmt_idx := N.div (Z.to_N idx) elmt_sz in
-                let byte_idx := (Z.to_N idx) mod elmt_sz in
-                match List.nth_error elts (N.to_nat elmt_idx) with
-                | Some elmt =>
-                    (* call dvalue_extract_byte recursively on the field *)
-                    dvalue_extract_byte elmt dt (Z.of_N byte_idx)
-                | None =>
-                    raise_error "dvalue_extract_byte: more fields in dvalue than in dtyp."
-                end
-            | _ =>
-                raise_error "dvalue_extract_byte: type mismatch on DVALUE_Vector."
-            end
-        end.
-    Proof.
-      induction dv.
-      1-12: cbn; reflexivity.
-    Admitted.
-
-    (* Taking a byte out of a dvalue...
-
-      Unlike UVALUE_ExtractByte, I don't think this needs an sid
-      (store id). There should be no nondeterminism in this value. *)
-    Inductive dvalue_byte : Type :=
-    | DVALUE_ExtractByte (dv : dvalue) (dt : dtyp) (idx : N) : dvalue_byte
-    .
-
-    Definition dvalue_byte_value {M} `{Monad M} `{RAISE_ERROR M} `{RAISE_POISON M} `{RAISE_OOMABLE M} (db : dvalue_byte) : M Z
-      := match db with
-         | DVALUE_ExtractByte dv dt idx =>
-             dvalue_extract_byte dv dt (Z.of_N idx)
-         end.
-
-    Obligation Tactic := try Tactics.program_simpl; try solve [cbn; try lia].
-    Program Fixpoint dvalue_bytes_to_dvalue {M} `{Monad M} `{RAISE_ERROR M} `{RAISE_POISON M} `{RAISE_OOMABLE M} (dbs : list dvalue_byte) (dt : dtyp) {measure (dtyp_measure dt)} : M dvalue
-      := match dt with
-         | DTYPE_I sz =>
-             zs <- map_monad dvalue_byte_value dbs;;
-             match sz with
-             | 1 =>
-                 ret (DVALUE_I1 (concat_bytes_Z_vint zs))
-             | 8 =>
-                 ret (DVALUE_I8 (concat_bytes_Z_vint zs))
-             | 32 =>
-                 ret (DVALUE_I32 (concat_bytes_Z_vint zs))
-             | 64 =>
-                 ret (DVALUE_I64 (concat_bytes_Z_vint zs))
-             | _ => raise_error "Unsupported integer size."
-             end
-         | DTYPE_IPTR =>
-             zs <- map_monad dvalue_byte_value dbs;;
-             val <- lift_OOMABLE DTYPE_IPTR (IP.from_Z (concat_bytes_Z zs));;
-             ret (DVALUE_IPTR val)
-         | DTYPE_Pointer =>
-             (* TODO: not sure if this should be wildcard provenance.
-                TODO: not sure if this should truncate iptr value...
-              *)
-             (* TODO: not sure if this should be lazy OOM or not *)
-             zs <- map_monad dvalue_byte_value dbs;;
-             match int_to_ptr (concat_bytes_Z zs) wildcard_prov with
-             | NoOom a => ret (DVALUE_Addr a)
-             | Oom msg => raise_oomable DTYPE_Pointer
-             end
-         | DTYPE_Void =>
-             raise_error "dvalue_bytes_to_dvalue on void type."
-         | DTYPE_Half =>
-             raise_error "dvalue_bytes_to_dvalue: unsupported DTYPE_Half."
-         | DTYPE_Float =>
-             zs <- map_monad dvalue_byte_value dbs;;
-             ret (DVALUE_Float (Float32.of_bits (concat_bytes_Z_vint zs)))
-         | DTYPE_Double =>
-             zs <- map_monad dvalue_byte_value dbs;;
-             ret (DVALUE_Double (Float.of_bits (concat_bytes_Z_vint zs)))
-         | DTYPE_X86_fp80 =>
-             raise_error "dvalue_bytes_to_dvalue: unsupported DTYPE_X86_fp80."
-         | DTYPE_Fp128 =>
-             raise_error "dvalue_bytes_to_dvalue: unsupported DTYPE_Fp128."
-         | DTYPE_Ppc_fp128 =>
-             raise_error "dvalue_bytes_to_dvalue: unsupported DTYPE_Ppc_fp128."
-         | DTYPE_Metadata =>
-             raise_error "dvalue_bytes_to_dvalue: unsupported DTYPE_Metadata."
-         | DTYPE_X86_mmx =>
-             raise_error "dvalue_bytes_to_dvalue: unsupported DTYPE_X86_mmx."
-         | DTYPE_Array sz t =>
-             let sz := sizeof_dtyp t in
-             elt_bytes <- lift_err_RAISE_ERROR (split_every sz dbs);;
-             elts <- map_monad (fun es => dvalue_bytes_to_dvalue es t) elt_bytes;;
-             ret (DVALUE_Array elts)
-         | DTYPE_Vector sz t =>
-             let sz := sizeof_dtyp t in
-             elt_bytes <- lift_err_RAISE_ERROR (split_every sz dbs);;
-             elts <- map_monad (fun es => dvalue_bytes_to_dvalue es t) elt_bytes;;
-             ret (DVALUE_Vector elts)
-         | DTYPE_Struct fields =>
-             match fields with
-             | [] => ret (DVALUE_Struct []) (* TODO: Not 100% sure about this. *)
-             | (dt::dts) =>
-                 let sz := sizeof_dtyp dt in
-                 let init_bytes := take sz dbs in
-                 let rest_bytes := drop sz dbs in
-                 f <- dvalue_bytes_to_dvalue init_bytes dt;;
-                 rest <- dvalue_bytes_to_dvalue rest_bytes (DTYPE_Struct dts);;
-                 match rest with
-                 | DVALUE_Struct fs =>
-                     ret (DVALUE_Struct (f::fs))
-                 | _ =>
-                     raise_error "dvalue_bytes_to_dvalue: DTYPE_Struct recursive call did not return a struct."
-                 end
-             end
-         | DTYPE_Packed_struct fields =>
-             match fields with
-             | [] => ret (DVALUE_Packed_struct []) (* TODO: Not 100% sure about this. *)
-             | (dt::dts) =>
-                 let sz := sizeof_dtyp dt in
-                 let init_bytes := take sz dbs in
-                 let rest_bytes := drop sz dbs in
-                 f <- dvalue_bytes_to_dvalue init_bytes dt;;
-                 rest <- dvalue_bytes_to_dvalue rest_bytes (DTYPE_Struct dts);;
-                 match rest with
-                 | DVALUE_Packed_struct fs =>
-                     ret (DVALUE_Packed_struct (f::fs))
-                 | _ =>
-                     raise_error "dvalue_bytes_to_dvalue: DTYPE_Packed_struct recursive call did not return a struct."
-                 end
-             end
-         | DTYPE_Opaque =>
-             raise_error "dvalue_bytes_to_dvalue: unsupported DTYPE_Opaque."
-         end.
-    Next Obligation.
-      pose proof dtyp_measure_gt_0 dt.
-      cbn.
-      unfold list_sum.
-      lia.
-    Qed.
-    Next Obligation.
-      pose proof dtyp_measure_gt_0 dt.
-      cbn.
-      unfold list_sum.
-      lia.
-    Qed.
-
-    Lemma dvalue_bytes_to_dvalue_equation
-      {M} `{HM : Monad M} `{RE: RAISE_ERROR M} `{RP: RAISE_POISON M} `{RO: RAISE_OOMABLE M} (dbs : list dvalue_byte) (dt : dtyp) :
-      @dvalue_bytes_to_dvalue M HM RE RP RO dbs dt =
-        match dt with
-        | DTYPE_I sz =>
-            zs <- map_monad dvalue_byte_value dbs;;
-            match sz with
-            | 1 =>
-                ret (DVALUE_I1 (concat_bytes_Z_vint zs))
-            | 8 =>
-                ret (DVALUE_I8 (concat_bytes_Z_vint zs))
-            | 32 =>
-                ret (DVALUE_I32 (concat_bytes_Z_vint zs))
-            | 64 =>
-                ret (DVALUE_I64 (concat_bytes_Z_vint zs))
-            | _ => raise_error "Unsupported integer size."
-            end
-        | DTYPE_IPTR =>
-            zs <- map_monad dvalue_byte_value dbs;;
-            val <- lift_OOMABLE DTYPE_IPTR (IP.from_Z (concat_bytes_Z zs));;
-            ret (DVALUE_IPTR val)
-        | DTYPE_Pointer =>
-            (* TODO: not sure if this should be wildcard provenance.
-                TODO: not sure if this should truncate iptr value...
-             *)
-            (* TODO: not sure if this should be lazy OOM or not *)
-            zs <- map_monad dvalue_byte_value dbs;;
-            match int_to_ptr (concat_bytes_Z zs) wildcard_prov with
-            | NoOom a => ret (DVALUE_Addr a)
-            | Oom msg => raise_oomable DTYPE_Pointer
-            end
-        | DTYPE_Void =>
-            raise_error "dvalue_bytes_to_dvalue on void type."
-        | DTYPE_Half =>
-            raise_error "dvalue_bytes_to_dvalue: unsupported DTYPE_Half."
-        | DTYPE_Float =>
-            zs <- map_monad dvalue_byte_value dbs;;
-            ret (DVALUE_Float (Float32.of_bits (concat_bytes_Z_vint zs)))
-        | DTYPE_Double =>
-            zs <- map_monad dvalue_byte_value dbs;;
-            ret (DVALUE_Double (Float.of_bits (concat_bytes_Z_vint zs)))
-        | DTYPE_X86_fp80 =>
-            raise_error "dvalue_bytes_to_dvalue: unsupported DTYPE_X86_fp80."
-        | DTYPE_Fp128 =>
-            raise_error "dvalue_bytes_to_dvalue: unsupported DTYPE_Fp128."
-        | DTYPE_Ppc_fp128 =>
-            raise_error "dvalue_bytes_to_dvalue: unsupported DTYPE_Ppc_fp128."
-        | DTYPE_Metadata =>
-            raise_error "dvalue_bytes_to_dvalue: unsupported DTYPE_Metadata."
-        | DTYPE_X86_mmx =>
-            raise_error "dvalue_bytes_to_dvalue: unsupported DTYPE_X86_mmx."
-        | DTYPE_Array sz t =>
-            let sz := sizeof_dtyp t in
-            elt_bytes <- lift_err_RAISE_ERROR (split_every sz dbs);;
-            elts <- map_monad (fun es => dvalue_bytes_to_dvalue es t) elt_bytes;;
-            ret (DVALUE_Array elts)
-        | DTYPE_Vector sz t =>
-            let sz := sizeof_dtyp t in
-            elt_bytes <- lift_err_RAISE_ERROR (split_every sz dbs);;
-            elts <- map_monad (fun es => dvalue_bytes_to_dvalue es t) elt_bytes;;
-            ret (DVALUE_Vector elts)
-        | DTYPE_Struct fields =>
-            match fields with
-            | [] => ret (DVALUE_Struct []) (* TODO: Not 100% sure about this. *)
-            | (dt::dts) =>
-                let sz := sizeof_dtyp dt in
-                let init_bytes := take sz dbs in
-                let rest_bytes := drop sz dbs in
-                f <- dvalue_bytes_to_dvalue init_bytes dt;;
-                rest <- dvalue_bytes_to_dvalue rest_bytes (DTYPE_Struct dts);;
-                match rest with
-                | DVALUE_Struct fs =>
-                    ret (DVALUE_Struct (f::fs))
-                | _ =>
-                    raise_error "dvalue_bytes_to_dvalue: DTYPE_Struct recursive call did not return a struct."
-                end
-            end
-        | DTYPE_Packed_struct fields =>
-            match fields with
-            | [] => ret (DVALUE_Packed_struct []) (* TODO: Not 100% sure about this. *)
-            | (dt::dts) =>
-                let sz := sizeof_dtyp dt in
-                let init_bytes := take sz dbs in
-                let rest_bytes := drop sz dbs in
-                f <- dvalue_bytes_to_dvalue init_bytes dt;;
-                rest <- dvalue_bytes_to_dvalue rest_bytes (DTYPE_Struct dts);;
-                match rest with
-                | DVALUE_Packed_struct fs =>
-                    ret (DVALUE_Packed_struct (f::fs))
-                | _ =>
-                    raise_error "dvalue_bytes_to_dvalue: DTYPE_Packed_struct recursive call did not return a struct."
-                end
-            end
-        | DTYPE_Opaque =>
-            raise_error "dvalue_bytes_to_dvalue: unsupported DTYPE_Opaque."
-        end.
-    Proof.
-    Admitted.
-
     Definition uvalue_sid_match (a b : uvalue) : bool
       :=
       match a, b with
@@ -1602,7 +1101,7 @@ Module MakeBase (LP : LLVMParams) (MP : MemoryParams LP) (Byte : ByteModule LP.A
                 | Oom msg =>
                     lift_ue (raise_oom ("concretize_uvalueM OOM in Conv_ItoP: " ++ msg))
                 end
-            | Conv_Pure x => concretize_uvalueM x
+            | Conv_Pure x => ret x
             | Conv_Illegal s => lift_ue (raise_error s)
             end
 
@@ -1836,7 +1335,7 @@ Module MakeBase (LP : LLVMParams) (MP : MemoryParams LP) (Byte : ByteModule LP.A
                     | Oom msg =>
                         lift_ue (raise_oom ("concretize_uvalueM OOM in Conv_ItoP: " ++ msg))
                     end
-                | Conv_Pure x => concretize_uvalueM x
+                | Conv_Pure x => ret x
                 | Conv_Illegal s => lift_ue (raise_error s)
                 end
 
