src/coq/Semantics/MemoryParams.v
@@ -1,16 +1,20 @@
 From Vellvm Require Import
      Semantics.LLVMParams
      Semantics.GepM
-     Semantics.Memory.MemBytes.
+     Semantics.Memory.MemBytes
+     Semantics.Memory.DvalueBytes.
 
 Module Type MemoryParams (LP : LLVMParams).
   Declare Module GEP : GEPM LP.ADDR LP.PTOI LP.PROV LP.ITOP LP.IP LP.SIZEOF LP.Events.
   Declare Module BYTE_IMPL : ByteImpl LP.ADDR LP.IP LP.SIZEOF LP.Events.
+  Declare Module DVALUE_BYTES : DvalueByte LP.
 End MemoryParams.
 
-Module Make (LP' : LLVMParams) (GEP' : GEPM LP'.ADDR LP'.PTOI LP'.PROV LP'.ITOP LP'.IP LP'.SIZEOF LP'.Events) (BYTE_IMPL' : ByteImpl LP'.ADDR LP'.IP LP'.SIZEOF LP'.Events) : MemoryParams LP'
+Module Make (LP' : LLVMParams) (GEP' : GEPM LP'.ADDR LP'.PTOI LP'.PROV LP'.ITOP LP'.IP LP'.SIZEOF LP'.Events) (BYTE_IMPL' : ByteImpl LP'.ADDR LP'.IP LP'.SIZEOF LP'.Events) (DVALUE_BYTES' : DvalueByte LP') : MemoryParams LP'
 with Module GEP := GEP'
-with Module BYTE_IMPL := BYTE_IMPL'.
+with Module BYTE_IMPL := BYTE_IMPL'
+with Module DVALUE_BYTES := DVALUE_BYTES'.
   Module GEP := GEP'.
   Module BYTE_IMPL := BYTE_IMPL'.
+  Module DVALUE_BYTES := DVALUE_BYTES'.
 End Make.
